only simple_log_rel_structural_1 left

theories/simulang/simple_inv/adequacy.v
@@ -20,6 +20,9 @@ Global Instance subG_sbijΣ Σ :
   subG simpleΣ Σ → simpleGpreS Σ.
 Proof. solve_inG. Qed.
 
+Print gen_log_rel.
+Print log_rel.
+
 Lemma prog_rel_adequacy Σ `{!simpleGpreS Σ} (p_t p_s : prog):
   isat (∀ `(simpleGS Σ) gs,
     ⌜map_Forall (λ _ v, val_wf v) gs⌝ -∗
@@ -46,9 +49,126 @@ Proof.
   - iIntros (??) "$".
 Qed.
 
+Locate prog_ref.
+Locate ctx_ref.
+Print expr_wf.
+Print ctx_ref.
+Print log_rel.
 (** Adequacy for open terms. *)
 Theorem log_rel_adequacy Σ `{!simpleGpreS Σ} e_t e_s :
   (∀ `(simpleGS Σ), ⊢ log_rel e_t e_s) →
+  ctx_ref e_t e_s.
+Proof.
+  intros Hrel C fname x p Hpwf HCwf Hvars.
+  apply (prog_rel_adequacy Σ). eapply isat_intro.
+  iIntros (? gs Hgs) "_ _ _ _ !#".
+  iSplit.
+  { iApply big_sepM_intro. iIntros "!>" (???). iApply val_wf_sound. by apply: Hgs. }
+  iApply prog_rel_refl_insert.
+  - iModIntro. iApply log_rel_func; first done.
+    iApply log_rel_ctx; first done. iApply Hrel.
+  - iIntros "!# %f %fn %Hfn". destruct fn as [arg body].
+    destruct (Hpwf _ _ Hfn) as [Hfn_wf Hfn_vars].
+    iApply log_rel_func; first set_solver.
+    iApply log_rel_refl. done.
+Qed.
+
+
+Definition gen_log_rel_1 `{simpleGS Σ} e_t e_s  : iProp Σ :=
+  □ ∀ π (map : gmap string (val * val)) (gs : gmap string val),
+    target_globals (dom gs) -∗
+    source_globals (dom gs) ==∗
+    subst_map_rel val_rel (free_vars e_t ∪ free_vars e_s) map -∗
+    subst_map (fst <$> map) e_t ⪯{π} subst_map (snd <$> map) e_s
+      {{ λ v_t v_s, val_rel v_t v_s }}.
+
+Print log_rel_ctx.
+Check log_rel_ctx.
+Locate log_rel_ctx.
+Locate gen_log_rel_ctx.
+Locate log_rel_structural.
+
+Definition log_rel_structural_1 `{simpleGS Σ} : Prop := (∀ e_t e_s,
+   let head_t := expr_split_head e_t in
+   let head_s := expr_split_head e_s in
+   simulang_wf head_s.1 →
+   head_s.1 = head_t.1 →
+   ([∗list] e_t';e_s' ∈ head_t.2; head_s.2, gen_log_rel_1 e_t' e_s') -∗
+   gen_log_rel_1 e_t e_s).
+
+
+Theorem gen_log_rel_refl_1 `{simpleGS Σ} e :
+  log_rel_structural_1 →
+  gen_expr_wf simulang_wf e →
+  ⊢ gen_log_rel_1 e e.
+Proof.
+  intros He Hwf.
+  iInduction e as [ ] "IH" forall (Hwf); destruct Hwf; iApply He. 
+  all: try iDestruct ("IH" with "[%]") as "$".
+  all: try iDestruct ("IH1" with "[%]") as "$".
+  all: try iDestruct ("IH2" with "[%]") as "$".
+  all: naive_solver.
+Qed.
+
+Theorem simple_log_rel_structural_1 `{simpleGS Σ} : log_rel_structural_1.
+Proof.
+Admitted.
+  (* intros e_t e_s ?? Hwf Hs. iIntros "IH".
+  destruct e_s, e_t => //; simpl in Hs; simplify_eq.
+  all: try by iApply pure_log_rel_structural; unfold loc_rel_func_law, loc_rel_inj_law, loc_rel_offset_law; eauto using heapbij_loc_func, heapbij_loc_inj, heapbij_loc_shift, sim_bij_contains_globalbij.
+  all: try iDestruct "IH" as "[IH IH1]".
+  all: try iDestruct "IH1" as "[IH1 IH2]".
+  all: try iDestruct "IH2" as "[IH2 IH3]".
+  - (* Call *)
+    iApply (log_rel_call with "IH IH1").
+    iIntros (???). rewrite /= left_id. auto.
+  - (* Fork *)
+    iApply (log_rel_fork with "IH").
+    iIntros (?????) "Hsim Hfork". iApply (sim_fork with "(Hsim [//])").
+    iIntros (?). iApply (sim_wand with "[Hfork]"). { by iApply "Hfork". }
+    iIntros (??). rewrite /= left_id. auto.
+  - (* AllocN *)
+    iApply (log_rel_allocN with "IH IH1").
+    iIntros (n ??????) "Hv Hcont".
+    target_alloc l_t as "Hl_t" "Ha_t"; first done.
+    source_alloc l_s as "Hl_s" "Ha_s"; first done.
+    iApply (sim_bij_insertN with "Ha_t Ha_s Hl_t Hl_s [Hv]"); [lia | by rewrite length_replicate.. | | ].
+    { iDestruct "Hv" as "#Hv".
+      rewrite big_sepL2_replicate_l; last by rewrite length_replicate.
+      generalize (Z.to_nat n) => n'.
+      iInduction n' as [] "IHn"; cbn; first done. iFrame "Hv IHn".
+    }
+    by iApply "Hcont".
+  - (* FreeN *)
+    iApply (log_rel_freeN with "IH IH1").
+    iIntros (???????) "Hv Hcont". sim_free. by iApply "Hcont".
+  - (* Load *)
+    iApply (log_rel_load with "IH").
+    iIntros (?????) "Hv Hcont". iApply (sim_bij_load with "Hv"). iIntros (??). by iApply "Hcont".
+  - (* Store *)
+    iApply (log_rel_store with "IH IH1").
+    iIntros (???????) "Hl Hv Hcont". iApply (sim_bij_store with "Hl Hv"). by iApply "Hcont".
+Qed. *)
+
+Corollary log_rel_ctx `{simpleGS Σ} C e_t e_s :
+  ctx_wf C →
+  gen_log_rel_1 e_t e_s -∗ gen_log_rel_1 (fill_ctx C e_t) (fill_ctx C e_s).
+Proof.
+  intros Hwf. iInduction (C) as [ | Ci C] "IH" using rev_ind; first by eauto.
+  iIntros "Hrel".
+  rewrite ->gen_ctx_wf_snoc in Hwf. destruct Hwf as [Kwf [Hewf Hiwf]].
+  iSpecialize ("IH" with "[//] Hrel").
+  rewrite !fill_ctx_app /=.
+  pose proof (simple_log_rel_structural_1) as He.
+  destruct Ci; simpl; iApply He => //=; iFrame "IH".
+  all: move: Hiwf; rewrite /= ?Forall_cons ?Forall_nil => Hiwf.
+  all: repeat iSplit; try done.
+  all: iApply gen_log_rel_refl_1; [done|].
+  all: naive_solver.
+Qed.
+
+Theorem log_rel_adequacy_1 Σ `{!simpleGpreS Σ} e_t e_s :
+  (∀ `(simpleGS Σ), ⊢ gen_log_rel_1 e_t e_s) →
   ctx_ref e_t e_s.
 Proof.
   intros Hrel C fname x p Hpwf HCwf Hvars.
