theories/simulang/simple_inv/examples/uberobj/lang_core.v
@@ -8,6 +8,10 @@ From iris.prelude Require Import options.
 From simuliris.simulang Require Import hoare behavior.
 From simuliris.simulang.simple_inv Require Import inv adequacy.
 
+Lemma union_empty_inv `{Countable A} (X Y : gset A) :
+  X ∪ Y = ∅ → X = ∅ ∧ Y = ∅.
+Proof. intros H1; set_solver. Qed.
+
 Definition hl_halted (e: expr) : option val := to_val e.
 
 Definition hl_at_external (e: expr) : option (string * val) :=
@@ -58,22 +62,22 @@ Section specs.
           prim_step functions e σ e' σ' efs ->
           hl_prim_step e σ e' σ'.
 
+  Notation uobj_id := nat.
   (* compartmentally pre-allocated heap space for uids *)
   Variable heap_by_uid : uobj_id -> list loc.  
-  Variable uid : uobj_id.
   (* fname -> (isCasm func * (pre-cond, post-cond)) *)
   Variable ext_funcs : string -> option (bool * ((state -> Prop) * (state -> Prop))). 
 
-  Definition R_relation (m: state) (m': state) (modified: bool) : Prop :=
+  Definition R_relation (uid: uobj_id) (m: state) (m': state) (modified: bool) : Prop :=
     closed (heap_by_uid uid) m' 
     /\ subseteq (dom m.(heap)) (dom m'.(heap))
     /\ (not modified -> forall l, In l (heap_by_uid uid) -> m.(heap) !! l = m'.(heap) !! l).
 
-  Inductive respecting_the_specs (e : expr) (m : state) (Q : state -> Prop) : Prop :=
+  Inductive respecting_the_specs (uid: uobj_id) (e : expr) (m : state) (Q : state -> Prop) : Prop :=
     | rts_base : 
-      forall m', R_relation m m' false ->
+      forall m', R_relation uid m m' false ->
       (* internal steps *)
-      ((forall (e' : expr) (m'' : state), hl_prim_step e m' e' m'' -> respecting_the_specs e' m'' Q )
+      ((forall (e' : expr) (m'' : state), hl_prim_step e m' e' m'' -> respecting_the_specs uid e' m'' Q )
         (* halted case *)
         /\ (not (eq (hl_halted e) None) -> Q m')
         (* external call case *)
@@ -82,11 +86,11 @@ Section specs.
           hl_at_external e = Some (fname, argv)
           -> Some (is_casm, (pre_spec, post_spec) ) = ext_funcs fname
           -> pre_spec m'
-          -> R_relation m' m'' is_casm
+          -> R_relation uid m' m'' is_casm
           -> post_spec m''
           -> hl_after_external (Some vret) e = Some e'
-          -> respecting_the_specs e' m Q) 
-      ) -> respecting_the_specs e m Q.
+          -> respecting_the_specs uid e' m Q) 
+      ) -> respecting_the_specs uid e m Q.
 
   (* =====================================================================================
                                     memory mapping 
@@ -145,14 +149,156 @@ Section specs.
       ∗ (mem_points_to_s s_mem.(heap)) 
       ∗ (mem_points_to_t t_mem.(heap)))%I.
 
-  Lemma preservation_of_respecting_the_specs Q_s Q_t :
-    Q_t = build_target_specification Q_s ->
-    forall s_exp t_exp (s_mem : state) (t_mem : state),
-      (⊢ {{{ mem_equiv_rel s_mem t_mem }}} 
-          t_exp ⪯[uid] s_exp
-        {{{ mem_equiv_post_rel }}})
-      -> respecting_the_specs s_exp s_mem Q_s
-      -> respecting_the_specs t_exp t_mem Q_t.
+  Lemma subst_map_with_no_free_vars :
+    forall e map,
+      free_vars e = ∅ ->
+      subst_map map e = e.
   Proof.
+    intros e map HNoFreeVars.
+    induction e.
+    - simpl. reflexivity.
+    - unfold free_vars in HNoFreeVars. inversion HNoFreeVars.
+    - simpl. reflexivity.
+    - simpl. inversion HNoFreeVars.
+      apply union_empty_inv in H0. destruct H0 as [H1 H2].
+      apply IHe1 in H1. admit.
+    - simpl. inversion HNoFreeVars.
+      apply union_empty_inv in H0. destruct H0 as [H1 H2].
+      apply IHe1 in H1. apply IHe2 in H2.
+      rewrite H1. rewrite H2. reflexivity.
+    - simpl. inversion HNoFreeVars.
+      apply IHe in H0. rewrite H0. reflexivity.
+    - simpl. inversion HNoFreeVars.
+      apply union_empty_inv in H0. destruct H0 as [H1 H2].
+      apply IHe1 in H1. apply IHe2 in H2.
+      rewrite H1. rewrite H2. reflexivity.
+    - simpl. inversion HNoFreeVars.
+      apply union_empty_inv in H0. destruct H0 as [H12 H3].
+      apply union_empty_inv in H12. destruct H12 as [H1 H2].
+      apply IHe1 in H1. apply IHe2 in H2. apply IHe3 in H3.
+      rewrite H1. rewrite H2. rewrite H3. reflexivity.
+    - simpl. inversion HNoFreeVars.
+      apply union_empty_inv in H0. destruct H0 as [H1 H2].
+      apply IHe1 in H1. apply IHe2 in H2.
+      rewrite H1. rewrite H2. reflexivity.
+    - simpl. inversion HNoFreeVars.
+      apply union_empty_inv in H0. destruct H0 as [H1 H2].
+      apply IHe1 in H1. apply IHe2 in H2.
+      rewrite H1. rewrite H2. reflexivity.
+    - simpl. inversion HNoFreeVars.
+      apply IHe in H0. rewrite H0. reflexivity.
+    - simpl. inversion HNoFreeVars.
+      apply IHe in H0. rewrite H0. reflexivity.
+    - simpl. inversion HNoFreeVars.
+      apply IHe in H0. rewrite H0. reflexivity.
+    - simpl. inversion HNoFreeVars.
+      apply IHe in H0. rewrite H0. reflexivity.
+    - simpl. inversion HNoFreeVars.
+      apply union_empty_inv in H0. destruct H0 as [H12 H3].
+      apply union_empty_inv in H12. destruct H12 as [H1 H2].
+      apply IHe1 in H1. rewrite H1. admit.
+    - simpl. inversion HNoFreeVars.
+      apply IHe in H0. rewrite H0. reflexivity.
+    - simpl. inversion HNoFreeVars.
+      apply union_empty_inv in H0. destruct H0 as [H1 H2].
+      apply IHe1 in H1. apply IHe2 in H2.
+      rewrite H1. rewrite H2. reflexivity.
+    - simpl. inversion HNoFreeVars.
+      apply union_empty_inv in H0. destruct H0 as [H1 H2].
+      apply IHe1 in H1. apply IHe2 in H2.
+      rewrite H1. rewrite H2. reflexivity.
+    - simpl. inversion HNoFreeVars.
+      apply IHe in H0. rewrite H0. reflexivity.
+    - simpl. inversion HNoFreeVars.
+      apply union_empty_inv in H0. destruct H0 as [H1 H2].
+      apply IHe1 in H1. apply IHe2 in H2.
+  Admitted.
+
+  Locate sim_expr.
+  Locate sim.
+  Locate unseal.
+  Search sim_expr.
+  Search sim_expr_stutter.
+  Locate "{{".
+  Print sim.
+  Locate subst_map_rel.
+  Locate free_vars.
+  Locate val_rel.
+  Locate "[{".
+  Print state.
+  Search "sim_expr".
+  Print state.
+  Locate log_rel.
+  Locate sim_def.
+  Locate prog.
+  Print func.
+  Lemma preservation_of_respecting_the_specs :
+    forall Q_s Q_t,
+      Q_t = build_target_specification Q_s ->
+      forall s_exp t_exp (s_mem : state) (t_mem : state),
+        (* there should be no dynamic heap of state.used_dyn_blocks (as we do not support dynamic allocations).
+           but only paired global static heap of state.globals which is initialized at the begining of the program *)
+        equivalence s_mem t_mem /\ s_mem.(used_dyn_blocks) = ∅ /\ t_mem.(used_dyn_blocks) = ∅
+        (* well-formedness of the program, there should be no free variables, e.g., variables introduced by let *)
+        /\ free_vars t_exp = ∅ /\ free_vars s_exp = ∅
+        -> forall uid,
+            (⊢ ∀ uid (map : gmap string (val * val)), 
+              {{{ mem_equiv_rel s_mem t_mem }}} 
+                t_exp ⪯[uid] s_exp
+              {{{ mem_equiv_post_rel }}})
+        -> respecting_the_specs uid s_exp s_mem Q_s
+        -> respecting_the_specs uid t_exp t_mem Q_t.
+  Proof.
+    intros Q_s Q_t HQt s_exp t_exp s_mem t_mem 
+          (HEquiv & HDynHeapEmpty_s & HDynHeapEmpty_t & HNoFreeVars_t & HNoFreeVars_s).
+    intros uid HQuadruple HResp_s.
+
+    assert (⊢ log_rel t_exp s_exp) as HLog_rel. {
+      unfold log_rel.
+      unfold sim.
+      simpl.
+      unfold sim_stutter.
+      unfold sim_def.
+ 
+      iModIntro.
+      iIntros (t_id map1).
+      unfold hoareSim in HQuadruple.
+      rewrite HNoFreeVars_s.
+      rewrite HNoFreeVars_t.
+      iIntros "HVal_rel".
+      iIntros "HTrue".
+
+      assert (subst_map (fst <$> map1) t_exp = t_exp) as HSubst_t. {
+        apply subst_map_with_no_free_vars. apply HNoFreeVars_t.
+      }
+      assert (subst_map (snd <$> map1) s_exp = s_exp) as HSubst_s. {
+        apply subst_map_with_no_free_vars. apply HNoFreeVars_s.
+      }
+      rewrite HSubst_t. rewrite HSubst_s.
+
+      unfold gen_log_rel.subst_map_rel.
+
+      iSpecialize (HQuadruple t_id).
+
+      (* sim_expr_decompose:
+        ∀ {PROP : bi} {BiBUpd0 : BiBUpd PROP} {BiAffine0 : BiAffine PROP} {BiPureForall0 : BiPureForall
+          PROP} {Λ : language} {s : simulirisGS PROPΛ} 
+          (e_t e_s : language.exprΛ) 
+          (Φ Ψ : language.expr Λ → language.expr Λ → PROP) (π : thread_id),
+          e_t ⪯{π} e_s [{ Ψ }] -∗
+          (∀ e_t0 e_s0 : language.expr Λ, Ψ e_t0 e_s0 -∗ e_t0 ⪯{π} e_s0 [{ Φ }]) -∗
+          e_t ⪯{π} e_s [{ Φ }] *)
+      
+      iSpecialize (HQuadruple t_id).
+     
+      admit.
+     }
+    destruct HResp_s as [s_mem' HR_relation_s HResp_s].
+    apply rts_base with (m' := t_mem).
+    - admit.
+    - repeat split.
+      + unfold hoareSim in HQuadruple.
+        unfold log_rel in HLog_rel.
+
   Admitted.
 End specs.
